@prefix : <#> .
@prefix rdf: <http://www.w3.org/1999/02/22-rdf-syntax-ns#> .
@prefix xsd: <http://www.w3.org/2001/XMLSchema#> .
@prefix rdfs: <http://www.w3.org/2000/01/rdf-schema#> .
@prefix dcterms: <http://purl.org/dc/terms/> .
@prefix owl: <http://www.w3.org/2002/07/owl#> .


<>
  dcterms:issued "2020-07-01"^^xsd:date ;
  dcterms:modified "2020-07-06"^^xsd:date ;
  rdfs:label "ShapeTree terms"@en .


# ShapeTree Class
#############################################################################
# Defines a tree of related resources which combine to enable some task
# see: https://shapetrees.github.io/specification/primer
#############################################################################
:ShapeTree
  a rdfs:Class ;
  rdfs:comment "Defines a composite data structure including a tree of resources and validation criteria"@en ;
  rdfs:isDefinedBy <> ;
  rdfs:label "Shape Tree"@en .

#
# Properties in domain of ShapeTree
#
:expectsType
  a owl:ObjectProperty ;
  rdfs:domain :ShapeTree ;
  rdfs:range [ owl:oneOf ( :Container :Resource ) ] ;
  rdfs:comment "Describes the expected type of resource the ShapeTree will validate against."@en ;
  rdfs:isDefinedBy <> ;
  rdfs:label "Expects Type"@en .

:contains
  a owl:ObjectProperty ;
  rdfs:domain :ShapeTree ;
  rdfs:range :ShapeTree  ;
  rdfs:comment "Links a ShapeTree to another ShapeTree that is directly contained within its planted Container"@en ;
  rdfs:isDefinedBy <> ;
  rdfs:label "Contains"@en .

:references
  a owl:ObjectProperty ;
  rdfs:domain :ShapeTree ;
  rdfs:range :ShapeTreeReference ;
  rdfs:isDefinedBy <> ;
  rdfs:comment "Links a ShapeTree to a ShapeTreeReference"@en ;
  rdfs:label "References"@en .

:shape
  a owl:ObjectProperty ;
  rdfs:domain :ShapeTree ;
  rdfs:comment "Links a ShapeTree to a Shape"@en ;
  rdfs:isDefinedBy <> ;
  rdfs:label "Shape"@en .

:supports
  a owl:ObjectProperty ;
  rdfs:domain :ShapeTree ;
  rdfs:range :ShapeTree ;
  rdfs:comment "Describes a relationship wherein a ShapeTree acts as a support for another, for purposes of indexing, aggregation, etc." ;
  rdfs:isDefinedBy <> ;
  rdfs:label "Supports"@en .

#
# Specific IRIs used by :contains predicate to define behavior
# when a matching ShapeTree with a URI Template is not found.
# These values can be combined, for example,
# :contains :AllowResources :AllowContainers :AllowNonRDFSources is equivalent to :AllowAll
# Example -- <#containerShapeTree> st:contains <#childShapeTree>, st:AllowResources
#
:AllowResources
  a :ShapeTree ;
  rdfs:comment "If no matching :contains ShapeTree is found, allow if the requested content is a :Resource"@en ;
  rdfs:isDefinedBy <> ;
  rdfs:label "Allow Resources"@en .

:AllowContainers
  a :ShapeTree ;
  rdfs:comment "If no matching :contains ShapeTree is found, allow if the requested content is a :Container"@en ;
  rdfs:isDefinedBy <> ;
  rdfs:label "Allow Containers"@en .

:AllowNonRDFSources
  a :ShapeTree ;
  rdfs:comment "If no matching :contains ShapeTree is found, only allow if the requested content is a :NonRDFResource"@en ;
  rdfs:isDefinedBy <> ;
  rdfs:label "Allow NonRDFSources"@en .

:AllowAll
  a :ShapeTree ;
  rdfs:comment "If no matching :contains ShapeTree is found, allow all types of unexpected content"@en ;
  rdfs:isDefinedBy <> ;
  rdfs:label "Allow All"@en .

:AllowNone
  a :ShapeTree ;
  rdfs:comment "If no matching :contains ShapeTree is found, do not allow any content"@en ;
  rdfs:isDefinedBy <> ;
  rdfs:label "Allow None"@en .

# Container IRI (maps to ldp:Container)
#############################################################################
# An IRI that represents a generalized container used in a ShapeTree
#############################################################################
:Container
  rdfs:comment "Describes a generalized container within a ShapeTree ecosystem"@en ;
  rdfs:isDefinedBy <> ;
  rdfs:label "Container"@en .


# Resource IRI (maps to ldp:Resource)
#############################################################################
# An IRI that represents a generalized resource used in a ShapeTree
#############################################################################
:Resource
  rdfs:comment "Describes a generalized RDF resource (non-container) within a ShapeTree ecosystem"@en ;
  rdfs:isDefinedBy <> ;
  rdfs:label "Resource"@en .

# NonRDFResource IRI (maps to ldp:NonRDFSource)
#############################################################################
# An IRI that represents a generalized resource used in a ShapeTree
#############################################################################
:NonRDFResource
  rdfs:comment "Describes a generalized non RDF / binary content within a ShapeTree ecosystem"@en ;
  rdfs:isDefinedBy <> ;
  rdfs:label "Non-RDF Resource"@en .


# ShapeTreeReference class
#############################################################################
# A ShapeTreeReference provides the necessary context to associate instance
# data between related ShapeTrees via a ShapePath
#############################################################################
:ShapeTreeReference
  a rdfs:Class ;
  rdfs:comment "Describes how a ShapeTree references another ShapeTree via a ShapePath"@en ;
  rdfs:isDefinedBy <> ;
  rdfs:label "ShapeTreeReference"@en .

#
# Properties in domain of ShapeTreeReference
#
:viaShapePath
  a owl:DatatypeProperty ;
  rdfs:domain :ShapeTreeReference ;
  rdfs:range xsd:string ;
  rdfs:comment "Describes how one ShapeTree traverses its instance data to reach another ShapeTree"@en ;
  rdfs:isDefinedBy <> ;
  rdfs:label "Via ShapePath"@en .


#
# Properties in range of ShapeTreeDecoratorIndex
#
:hasShapeTreeDecoratorIndex
  a owl:ObjectProperty ;
  rdfs:range :ShapeTreeDecoratorIndex ;
  rdfs:isDefinedBy <> ;
  rdfs:label "Has ShapeTree Decorator Index"@en .

# ShapeTreeDecoratorIndex class
#############################################################################
# A ShapeTreeDecoratorIndex details a ShapeTree in a human-readable way.
# It is primarily used for use cases where a ShapeTree must be described to
# a user for purposes of authorization.
#############################################################################
:ShapeTreeDecoratorIndex
  a rdfs:Class ;
  rdfs:comment "Provides an index of SKOS poly-hierarchies which can be used to describe a ShapeTree"@en ;
  rdfs:isDefinedBy <> ;
  rdfs:label "ShapeTreeDecoratorIndex"@en .

# Properties in domain of ShapeTreeDecoratorIndex
#########################################################
:hasSet
  a owl:ObjectProperty ;
  rdfs:domain :ShapeTreeDecoratorIndex ;
  rdfs:range :ShapeTreeDecoratorSet ;
  rdfs:comment "Links between a ShapeTreeDecoratorIndex and a ShapeTreeDecoratorSet"@en ;
  rdfs:isDefinedBy <> ;
  rdfs:label "Has Set"@en .

:defaultLanguage
  a owl:ObjectProperty ;
  rdfs:domain :ShapeTreeDecoratorIndex ;
  rdfs:range xsd:language ;
  rdfs:comment "Defines default language for use with shape tree decorator when none exist matching user preferences"@en ;
  rdfs:isDefinedBy <> ;
  rdfs:label "Default language"@en .


# ShapeTreeDecoratorSet class
#############################################################################
# A ShapeTreeDecoratorSet details a set of ShapeTreeDecoratorResource classes
# Primary use is grouping ShapeTreeDecoratorResource instances by a common
# discriminator such as language or intended audience
#############################################################################
:ShapeTreeDecoratorSet
  a rdfs:Class ;
  rdfs:comment "Groups a set of ShapeTreeDecoratorResource by a given discriminator"@en ;
  rdfs:isDefinedBy <> ;
  rdfs:label "ShapeTreeDecoratorSet"@en .

#
# Properties in domain of ShapeTreeDecoratorSet
#
:hasShapeTreeDecoratorResource
  a owl:ObjectProperty ;
  rdfs:domain :ShapeTreeDecoratorSet ;
  rdfs:range :ShapeTreeDecoratorResource ;
  rdfs:comment "Links between a ShapeTreeDecoratorSet and the decorator resource itself"@en ;
  rdfs:isDefinedBy <> ;
  rdfs:label "Has Decorator Resource"@en .

:usesLanguage
  a owl:ObjectProperty ;
  rdfs:domain :ShapeTreeDecoratorSeries ;
  rdfs:range xsd:language ;
  rdfs:comment "Describes the language used by associated ShapeTreeDecoratorResource"@en ;
  rdfs:isDefinedBy <> ;
  rdfs:label "Uses language"@en .

# ShapeTreeDecoratorResource class
#############################################################################
# A ShapeTreeDecoratorResource represents a SKOS-based resource which
# is made up of multiple st:ShapeTreeDecorator nodes that describe shape trees
#############################################################################
:ShapeTreeDecoratorResource
  a rdfs:Class ;
  rdfs:comment "Represents a SKOS-based resource which is made up of multiple st:ShapeTreeDecorator nodes that describe shape trees"@en ;
  rdfs:isDefinedBy <> ;
  rdfs:label "ShapeTreeDecoratorResource"@en .

# ShapeTreeDecorator class
#############################################################################
# A ShapeTreeDecorator represents a single descriptor of a shape tree
#############################################################################
:ShapeTreeDecorator
  a rdfs:Class ;
  rdfs:comment "A ShapeTreeDecorator represents a single descriptor of a shape tree"@en ;
  rdfs:isDefinedBy <> ;
  rdfs:label "ShapeTreeDecorator"@en .


# Properties in the range of ShapeTreeLocator
#########################################################
:hasShapeTreeLocator
  a owl:ObjectProperty ;
  rdfs:range :ShapeTreeLocator ;
  rdfs:comment "Represents the association between a subject an one or more ShapeTreeLocator"@en ;
  rdfs:isDefinedBy <> ;
  rdfs:label "Has ShapeTree Locator"@en .


# ShapeTreeLocator class
#############################################################################
# A ShapeTreeLocator describes a planted ShapeTree in a container with enough
# information to traverse from the current container to the root
#############################################################################
:ShapeTreeLocator
  a rdfs:Class ;
  rdfs:comment "Describes a planted ShapeTree in a container with enough information to traverse from the current container to the root"@en ;
  rdfs:isDefinedBy <> ;
  rdfs:label "ShapeTreeLocator"@en .

# Properties in domain of ShapeTreeLocator
#########################################################

:hasShapeTreeInstanceRoot
  a owl:ObjectProperty ;
  rdfs:domain :ShapeTreeLocator ;
  rdfs:comment "Represents the IRI of a root of a planted ShapeTree hierarchy"@en ;
  rdfs:isDefinedBy <> ;
  rdfs:label "Has ShapeTree Instance Root"@en .

:hasRootShapeTree
  a owl:ObjectProperty ;
  rdfs:domain :ShapeTreeLocator ;
  rdfs:range :ShapeTree ;
  rdfs:comment "Represents the ShapeTree that is planted at the root of the ShapeTree hierarchy.  For flat structures, hasRootShapeTree and hasShapeTree will be the same."@en ;
  rdfs:isDefinedBy <> ;
  rdfs:label "Has Root ShapeTree"@en .


################################################################
# A generalized predicate for linking a class to a ShapeTree
################################################################
:hasShapeTree
  a owl:ObjectProperty ;
  rdfs:range :ShapeTree ;
  rdfs:comment "Represents the IRI of a ShapeTree that is referenced by some subject"@en ;
  rdfs:isDefinedBy <> ;
  rdfs:label "Has ShapeTree Instance Root"@en .
